CTL.lean
@@ -1,5 +1,7 @@
-import «CTL».Basic
 import «CTL».Satisfaction
+import «CTL».Equivalence
+
+import «CTL».Basic
 import «CTL».Normal
 import «CTL».Checking
 import «CTL».Examples
